# Model Selection
Within this section, we will prove the properties of information criterion used
to select models. The framework for the derivations of information criteria
will be based upon the the following;

\[{Y_t} = \sum\limits_{i = 1}^p {{\phi _i}{Y_{t - i}} + {W_t}} ,{W_t}\mathop  \sim \limits^{iid} N\left( {0,{\sigma ^2}} \right)\]

The construction of a design matrix $X$ as follows: 
${\left( X \right)_{t,j}} = {X_{t,j}} = {Y_{t - j}}$
for $j = 1, \ldots, p$ and $t = p + 1, \ldots, n$.

If we let $\phi  = {\left[ {\begin{array}{*{20}{c}}
  {{\phi _1}}& \cdots &{{\phi _p}} 
\end{array}} \right]^T}$, then $\hat \phi  = {\left( {{X^T}X} \right)^{ - 1}}{X^T}Y$

where $Y = {\left[ {\begin{array}{*{20}{c}}
  {{Y_{p + 1}}}& \cdots &{{Y_n}} 
\end{array}} \right]^T} \Rightarrow Y = X\phi  + \varepsilon$

Define $\tilde \sigma _p^2 = \frac{1}{m}\sum\limits_{i = p + 1}^n {{{\left( {{Y_i} - {{\hat Y}_i}} \right)}^2}}$

${\hat Y_t} = \sum\limits_{i = 1}^P {{{\hat \phi }_i}{Y_{t - i}}}  = X\hat \phi$

and \[S_p^2 = \frac{1}{{n - p}}\sum\limits_{i = p + 1}^n {{{\left( {{Y_i} - {{\hat Y}_i}} \right)}^2}} \]

## Derivations of Information Criterion

Under the above definitions, we will procedure to derive both Mallow's Cp and AIC
model selection criteria. With a slight loss of generality, we will simplify the
derivations slightly by considering $X$ as a fixed matrix.

Define: \[C = E\left[ {{E_0}\left[ {\left\| {{Y_0} - \hat Y} \right\|_2^2} \right]} \right]\],
where $Y_o$ is independent copy of $Y$.

```{theorem}
\[C = E\left[ {\left\| {Y - \hat Y} \right\|_2^2} \right] + 2tr\left( {\cov\left( {Y,\hat Y} \right)} \right)\]
```

```{proof}
We begin by examining the norm:

\begin{align*}
  \left\| {Y - \hat Y} \right\|_2^2 &= \left\| {Y - X\hat \phi } \right\|_2^2 = {Y^T}Y + {{\hat \phi }^T}{X^T}X\phi  - 2{Y^T}X\hat \phi  \hfill \\
   &= {Y^T}Y + {{\hat \phi }^T}{X^T}X\phi  - 2{\left( {Y - X\hat \phi } \right)^T}X\hat \phi  \hfill \\ 
\end{align*}

So,

\[E\left[ {{E_0}\left[ {\left\| {Y_0 - \hat Y} \right\|_2^2} \right]} \right] = {E_0}\left[ {Y_0^TY} \right] - E\left[ {{{\hat \phi }^T}{X^T}X\hat \phi } \right] - 2E\left[ {{{\left( {{E_0}\left[ {{Y_0}} \right] - X\hat \phi } \right)}^T}X\hat \phi } \right]\]

Let ${C^*} = E\left[ {\left\| {Y - \hat Y} \right\|_2^2} \right] = E\left[ {{Y^T}Y} \right] - E\left[ {\hat \phi {X^T}X\hat \phi } \right] - 2E\left[ {{{\left( {Y - X\hat \phi } \right)}^T}X\hat \phi } \right]$

Therefore,

\begin{align*}
  C - {C^*} &= 2E\left[ {{{\left( {Y - {E_0}\left[ {{Y_0}} \right]} \right)}^T}X\hat \phi } \right]\overbrace  = ^{\left( * \right)}2tr\left( {\cov\left( {{Y_0} - {E_0}\left[ {{Y_0}} \right],X\hat \phi } \right)} \right) + 2tr\left( {E\left[ {y - {E_0}\left[ {{Y_0}} \right]} \right]E\left[ {X\hat \phi } \right]} \right) \hfill \\
   &= 2tr\left( {\cov\left( {Y,X\hat \phi } \right)} \right) = 2tr\left( {\cov\left( {Y,\hat Y} \right)} \right) \hfill \\ 
\end{align*}

$\left({*}\right)$ follows from:

\[E\left[ {{X^T}Z} \right] = E\left[ {tr\left( {{X^T}Z} \right)} \right] = E\left[ {tr\left( {Z{X^T}} \right)} \right] = tr\left( {\cov\left( {X,Z} \right)} \right) + tr\left( {E\left[ X \right]{E^T}\left[ Z \right]} \right)\]
```

```{theorem, name="Mallow Cp"}

The model selection criteria for Mallow Cp is defined to be:

\[{C_p} = \frac{{\left\| {Y - \hat Y} \right\|_2^2}}{{S_p^2}} - m + 2p\],

where $m = n-p$. The value of $m$ is associated with the "effective length".
```

```{proof}
If $\hat Y = X\hat \phi$ with a biased $X$, then

\begin{align*}
  tr\left( {\cov\left( {Y,\hat Y} \right)} \right) &= tr\left( {\cov\left( {Y,\underbrace {X{{\left( {{X^T}X} \right)}^{ - 1}}{X^T}}_{ = H}Y} \right)} \right) = tr\left( {\cov\left( {Y,Y} \right)H} \right) \hfill \\
   &= tr\left( {\operatorname{var} \left( Y \right)H} \right) = tr\left( {\operatorname{var} \left( {X\phi  + \varepsilon } \right)H} \right) = tr\left( {{\sigma ^2}IH} \right) = {\sigma ^2}tr\left( H \right) \hfill \\
   &= {\sigma ^2}p \hfill \\ 
\end{align*}

Therefore,

\[{{\tilde C}_p} = \left\| {Y - \hat Y} \right\|_2^2 + 2S_p^2p\]

such that \[E\left[ {{{\tilde C}_p}} \right] \approx C \text{ since } E\left[ {S_p^2} \right] = {\sigma ^2}\].

Thus, \[{C_p} = \frac{{{{\tilde C}_p}}}{{S_p^2}} - m\] 

or, equivalently,

\[{C_p} = \frac{{\left\| {Y - \hat Y} \right\|_2^2}}{{S_p^2}} - m + 2p\]
```


```{definition, label="kldc", name = "Kullback-Leibler Divergence Criterion"}
The Kullbackâ€“Leibler divergence criterion
given by:

\[KL = \frac{1}{m}E\left[ {{E_0}\left[ {\log \left( {\frac{{f\left( {{Y_0}|{\theta _0}} \right)}}{{f\left( {{Y_0}|\hat \theta } \right)}}} \right)} \right]} \right]\]

where $\hat \theta$ is the estimated parameters on $y$, $m$ is the length of $y$, and $\theta_0$ is the true parameter.
```

```{theorem, name = "Akaike information criterion (AIC)"}
The Akaike information criterion (AIC) is based upon \@ref(def:kldc) and is 
given by:

\[AIC = \log \left( {\hat \sigma _p^2} \right) + \frac{{2\left( {p + 1} \right)}}{m}\]
```


```{proof}
We have:

\begin{align*}
  f\left( {Y|\theta } \right) &= {\left( {2\pi } \right)^{ = \frac{m}{2}}}{\left| {{\sigma ^2}I} \right|^{ - \frac{1}{2}}}\exp \left( { - \frac{1}{2}{{\left( {Y - X\phi } \right)}^T}{{\left( {{\sigma ^2}I} \right)}^{ - 1}}\left( {Y - X\phi } \right)} \right) \hfill \\
   &= {\left( {2\pi } \right)^{ = \frac{m}{2}}}{\left( {{\sigma ^2}} \right)^{ - \frac{m}{2}}}\exp \left( { - \frac{1}{{2{\sigma ^2}}}{{\left( {Y - X\phi } \right)}^T}\left( {Y - X\phi } \right)} \right) \hfill \\
\end{align*}

where $m = n-p$.

From here, we apply \@ref(def:kldc) to get:
\begin{align*}
  &\frac{1}{m}E\left[ {{E_0}\left[ {\log \left( {\frac{{f\left( {{Y_0}|{\theta _0}} \right)}}{{f\left( {{Y_0}|\hat \theta } \right)}}} \right)} \right]} \right] \\
  &= \frac{1}{m}E\left[ {{E_0}\left[ {\log \left( {{{\left( {\frac{{\sigma _0^2}}{{\hat \sigma _p^2}}} \right)}^{ - \frac{m}{2}}}} \right) + \log \left( {\frac{{\exp \left( { - \frac{1}{{2{\sigma ^2}}}{{\left( {{Y_0} - X{\phi _0}} \right)}^T}\left( {{Y_0} - X{\phi _0}} \right)} \right)}}{{\exp \left( { - \frac{1}{{2{{\hat \sigma }^2}}}{{\left( {{Y_0} - X\hat \phi } \right)}^T}\left( {{Y_0} - X\hat \phi } \right)} \right)}}} \right)} \right]} \right] \hfill \\
   &= \underbrace {\frac{1}{m}\left( { - \frac{m}{2}} \right)E\left[ {{E_0}\left[ {\frac{{\sigma _0^2}}{{\hat \sigma _p^2}}} \right]} \right]}_{\left( 1 \right)} - \underbrace {\frac{1}{{2\sigma _0^2m}}{E_0}\left[ {{{\left( {{Y_0} - X{\phi _0}} \right)}^T}\left( {{Y_0} - X{\phi _0}} \right)} \right]}_{\left( 2 \right)} \\
   &+ \underbrace {\frac{1}{{2m}}E\left[ {\frac{1}{{2\hat \sigma _p^2}}{E_0}\left[ {{{\left( {{Y_0} - X\hat \phi } \right)}^T}\left( {{Y_0} - X\hat \phi } \right)} \right]} \right]}_{\left( 3 \right)} \hfill \\ 
\end{align*}

Treating each component piece wise yields:

\begin{align*}
  \left( 1 \right) &=  - \frac{1}{2}E\left[ {{E_0}\left[ {\frac{{\sigma _0^2}}{{\hat \sigma _p^2}}} \right]} \right] = \frac{1}{2}\left( {E\left[ {\log \left( {\hat \sigma _p^2} \right)} \right] - \log \left( {\sigma _0^2} \right)} \right) \hfill \\
  \left( 2 \right) &=  - \frac{1}{2}\left\{ {\frac{1}{{\sigma _0^2}}\underbrace {\frac{1}{m}{E_0}\left[ {{{\left( {{Y_0} - X{\phi _0}} \right)}^T}\left( {{Y_0} - X{\phi _0}} \right)} \right]}_{ = \sigma _0^2}} \right\} =  - \frac{1}{2} \hfill \\
  \left( 3 \right) &= \frac{1}{{2m}}E\left[ {\frac{1}{{\hat \sigma _p^2}}{E_0}\left[ {{{\left( {{Y_0} - X{\phi _0} - X\left( {\hat \phi  - {\phi _0}} \right)} \right)}^T}\left( {{Y_0} - X{\phi _0} - X\left( {\hat \phi  - {\phi _0}} \right)} \right)} \right]} \right] \hfill \\
   &= \frac{1}{{2m}}E\left[ {\frac{1}{{\hat \sigma _p^2}}\underbrace {{E_0}\left[ {{{\left( {{Y_0} - X{\phi _0}} \right)}^T}\left( {{Y_0} - X{\phi _0}} \right)} \right]}_{ = \sigma _0^2m}} \right] + \frac{1}{{2m}}E\left[ {\frac{1}{{\hat \sigma _p^2}}{E_0}\left[ {{{\left( {\hat \phi  - {\phi _0}} \right)}^T}{X^T}X\left( {\hat \phi  - {\phi _0}} \right)} \right]} \right] \hfill \\
   &- \underbrace {\frac{1}{m}E\left[ {\frac{1}{{\hat \sigma _p^2}}{E_0}\left[ {{{\left( {{Y_0} - X{\phi _0}} \right)}^T}\left( {X\left( {\hat \phi  - {\phi _0}} \right)} \right)} \right]} \right]}_{ = 0} \hfill \\
   &= \underbrace {\frac{1}{2}E\left[ {\frac{{\sigma _0^2}}{{\hat \sigma _p^2}}} \right]}_{\left( 4 \right)} + \underbrace {\frac{1}{{2m}}E\left[ {\frac{{\sigma _0^2}}{{\hat \sigma _p^2}}{E_0}\left[ {\frac{{{{\left( {\hat \phi  - {\phi _0}} \right)}^T}{X^T}X\left( {\hat \phi  - {\phi _0}} \right)}}{{\sigma _0^2}}} \right]} \right]}_{\left( 5 \right)}
\end{align*}

At this point, it would be helpful to recall the a few properties
regarding the $\chi^2$ distribution. In particular, note that:

\[{U_1} = \frac{{m\hat \sigma _p^2}}{{\sigma _0^2}} \sim \chi _{m - p}^2 , 
  {U_2} = \frac{{{{\left( {\hat \phi  - {\phi _0}} \right)}^T}{X^T}X\left( {\hat \phi  - {\phi _0}} \right)}}{{\sigma _0^2}} \sim \chi _p^2 \]

If $U \sim \chi _k^2$, then $E\left[ {\frac{1}{U}} \right] = \frac{1}{{K - 2}}$.

Lastly, note that $U_1$ and $U_2$ are independent. 

From these properties, we can derive the following:

\begin{align*}
  \left( 4 \right) &= \frac{1}{2}E\left[ {\frac{{\sigma _0^2}}{{\hat \sigma _p^2}}} \right] = \frac{m}{2}E\left[ {\frac{{\sigma _0^2}}{{m\hat \sigma _p^2}}} \right] = \frac{m}{2}\frac{1}{{\left( {m - p - 2} \right)}} = \frac{m}{{2\left( {m - p - 2} \right)}} \hfill \\ 
    \left( 5 \right) &= \frac{1}{2}E\left[ {\frac{{\sigma _0^2}}{{m\hat \sigma _p^2}}} \right]{E_0}\left[ {\frac{{{{\left( {\hat \phi  - {\phi _0}} \right)}^T}{X^T}X\left( {\hat \phi  - {\phi _0}} \right)}}{{\sigma _0^2}}} \right] = \frac{1}{2}\left( {\frac{1}{{m - p - 2}}} \right)\left( p \right) = \frac{p}{{2\left( {m - p - 2} \right)}} \hfill \\
\end{align*}

Having said this, we are now able to use both $\left( 4 \right)$ and $\left( 5 \right)$ to 
obtain $\left( 3 \right)$:

\[\left( 3 \right) = \left( 4 \right) + \left( 5 \right) = \frac{{p + m}}{{2\left( {m - p - 2} \right)}}\]

Therefore, we have:

\begin{align*}
\frac{1}{m}E\left[ {{E_0}\left[ {\log \left( {\frac{{f\left( {{Y_0}|{\theta _0}} \right)}}{{f\left( {{Y_0}|\hat \theta } \right)}}} \right)} \right]} \right] &= \left( 1 \right) + \left( 2 \right) + \left( 3 \right) \\
&= \frac{1}{2}\left( {E\left[ {\log \left( {\hat \sigma _p^2} \right)} \right] - \log \left( {\sigma _0^2} \right) - 1} \right) + \frac{{p + m}}{{2\left( {m - p - 2} \right)}}
\end{align*}

Note that the ${ - \log \left( {\sigma _0^2} \right) - 1}$ is constant
throughout the different models and is therefore not significant. Thus,

\[KL \propto E\left[ {\log \left( {\hat \sigma _p^2} \right)} \right] + \frac{{p + m}}{{\left( {m - p - 2} \right)}}\]

giving

\begin{align*}
  AICc &= \log \left( {\hat \sigma _p^2} \right) + \frac{{p + m}}{{\left( {m - p - 2} \right)}} \hfill \\
  AIC &= \log \left( {\hat \sigma _p^2} \right) + \frac{{2\left( {p + 1} \right)}}{m} \hfill \\ 
\end{align*}

since $\log \left( {\hat \sigma _p^2} \right)$ is an unbiased estimator of $E\left[ {\log \left( {\hat \sigma _p^2} \right)} \right]$.
```

## Properties of Model Selection

Consider multiple AR(p) models each with a different parameterization denoted
by:

$$\mathcal{M}_j: {Y_t} = \sum\limits_{i = 1}^j {{\phi _i}{Y_{t - i}}}  + {W_t}$$
Consider the following model selection criteria:


\begin{align*}
  AI{C_j} &= \log \left( {\hat \sigma _j^2} \right) + \frac{{2\left( {{p_j} + 1} \right)}}{m} \hfill \\
  BI{C_j} &= \log \left( {\hat \sigma _j^2} \right) + \frac{{\log \left( m \right){p_j}}}{m} \hfill \\
  H{Q_j}  &= \log \left( {\hat \sigma _j^2} \right) + \frac{{2\log \left( {\log \left( m \right)} \right){p_j}}}{m} \hfill \\ 
  Crit    &= \log \left( {\hat \sigma _j^2} \right) + \lambda \frac{p}{m}, \text{where }\lambda=2,\log(m),\log(\log(m))
\end{align*}

Note: \[\hat \sigma _j^2 = \frac{1}{m}\sum\limits_{i = {p_{j + 1}}}^m {{{\left( {{Y_i} - \hat Y_i^{\left( j \right)}} \right)}^2}} \]

In particular, $$Crit_j = Crit(\mathcal{M}_j)$$ and $\hat j = \mathop {\arg \min }\limits_{j = 1, \cdots ,J} {Crit_j}$ 
denote the best model.

The following properties hold:

1. $\mathop {\lim }\limits_{n \to \infty } P\left( {\hat j = {j_0}} \right) = 1$
2. $\mathop {\lim }\limits_{n \to \infty } P\left( {{L_n}\left( {\hat j} \right) = {L_n}\left( {{j_0}} \right)} \right)\mathop  \to \limits^P 1$ where
  ${L_n}\left( {{j_0}} \right) = \frac{1}{n}\left\| {\mu  - {{\hat Y}_j}} \right\|_2^2$ and $\mu  = E\left[ Y \right]$.

There are two cases two be wary about regarding the above properties.

The first is when $E\left[ {{{\hat Y}_{{j_0}}}} \right] = \mu$, then
for the BIC and HQ selection criteria both (1) + (2) hold. However, in the
case of AIC and Mallow Cp only (2) holds.

The converse, $E\left[ {{{\hat Y}_{{j_0}}}} \right] \neq \mu$, yields BIC and HQ
selection criteria having neither of the above properties. However, in the
case of AIC and Mallow Cp (2) condition still holds under some technical conditions.

## Model Selection Simulation Studies

Within this section, we hope to illustrate that the various properties of the
model selection criteria. In particular, the AIC and Mallow Cp predict the model
as the best model even though $j_0$ may not be a candidate whereas with BIC and HQ, 
will pick the right model with probability 1 as the sample size goes to infinity
when $j_0$ is a candidate.

Simulation omitted temporarily.