# Linear Processes

## The Backshift Operator

### Definition

The **Backshift Operator** is helpful when manipulating time series. When we 
backshift, we are changing the indices of the time series.
e.g. $t \rightarrow t-1$. The operator is defined as:

\[B{X_t} = {X_{t - 1}}\]

Backshifting on a constant, $c$, results in:

\[Bc = c\]

If we were to repeatedly apply the backshift operator, we would receive:

\[\begin{aligned}
  {B^2}{X_t} &= B\left( {B{X_t}} \right) \\
   &= B\left( {{X_{t - 1}}} \right) \\
   &= {X_{t - 2}} \\ 
\end{aligned}\]

We can generalize this behavior as:

$${B^k}{X_t} = {X_{t - k}}$$

The backshift operator is helpful for later decompositions in addition to making
differencing operations more straightforward.

The notation for the backshift operator changes depending on the author's 
preferences. An alternative way to denote a backshift operation given by $B$
is to use the lag operator $L$. The same conventions as discussed above apply
equally to the lag operator.

## Differencing Operator

*Definition:* **Differencing Operator**

The **Differencing Operator** is defined as the gradient symbol applied to a time series:
\[\nabla {X_t} = {X_t} - {X_{t - 1}}\]

The differencing operator is helpful when trying to remove trend from the data.
Many make an analogy between this operator and taking a first derivative of
a function.

We can take higher moments of differences by:
\[\begin{aligned}
  {\nabla ^2}{X_t} &= \nabla \left( {\nabla {X_t}} \right) \\
   &= \nabla \left( {{X_t} - {X_{t - 1}}} \right) \\
   &= \left( {{X_t} - {X_{t - 1}}} \right) - \left( {{X_{t - 1}} - {X_{t - 2}}} \right) \\
   &= {X_t} - 2{X_{t - 1}} + {X_{t - 2}} \\ 
\end{aligned} \]

So, the difference operator has the following properties:
\[\begin{aligned}
  {\nabla ^k}{X_t} &= {\nabla ^{k - 1}} \left( {\nabla {X_t}}\right) \\
  {\nabla ^1}{X_t} &= \nabla {X_t} \\ 
\end{aligned} \]

Notice, within the difference operation, we are backshifting the timeseries.

If we rewrite the difference operator to use the backshift operator, we receive:
\[\nabla {X_t} = {X_t} - {X_{t - 1}} = \left( {1 - B} \right){X_t}\]

This holds for later incarnations as well:
\[\begin{aligned}
  {\nabla ^2}{X_t} &= {X_t} - 2{X_{t - 1}} + {X_{t - 2}} \\
   &= \left( {1 - B} \right)\left( {1 - B} \right){X_t} \\
   &= {\left( {1 - B} \right)^2}{X_t} \\ 
\end{aligned} \]

Thus, we can generalize this to:
\[{\nabla ^k}{X_t} = {\left( {1 - B} \right)^k}{X_t}\]

### Seasonal Differencing Operator

With a slight change to the difference operator, a seasonal difference can be
applied by using a backshift greater than 1:

\[{\nabla _s}{X_t} = {X_t} - {X_{t - s}} = \left( {1 - B_s} \right){X_t}\]

In a similar vein, the above is able to be differenced by:

\[{\nabla ^k_s}{X_t} = {\left( {1 - B_s} \right)^k}{X_t}\]

## Linear Process

### Definition

A time series, $(X_t)$, is defined to be a linear process if it can be expressed
as a linear combination of white noise by:

\[{X_t} = \mu + \sum\limits_{j =  - \infty }^\infty  {{\psi _j}{W_{t - j}}} \]

where $W_t \sim WN(0, \sigma^2)$ and $\sum\limits_{j =  - \infty }^\infty  {\left| {{\psi _j}} \right|}  < \infty$.
Note, the later assumption is required to ensure that the series has a limit. 
Furthermore, the set of coefficients \[{\{ {\psi _j}\} _{j =  - \infty , \cdots ,\infty }}\]
can be viewed as linear filter. These coefficients do not have to be all equal
nor symmetric as later examples will show. Generally, the properties of a linear
process related to mean and variance are given by:

\[\begin{aligned}
\mu_{X} &= \mu \\
\gamma_{X}(h) &= \sigma _W^2\sum\limits_{j =  - \infty }^\infty  {{\psi _j}{\psi _{h + j}}}
\end{aligned}\]

The latter is derived from 

\[\begin{aligned}
  \gamma \left( h \right) &= Cov\left( {{x_t},{x_{t + h}}} \right) \\
   &= Cov\left( {\mu  + \sum\limits_{j =  - \infty }^\infty  {{\psi _j}{w_{t - j}}} ,\mu  + \sum\limits_{j =  - \infty }^\infty  {{\psi _j}{w_{t + h - j}}} } \right) \\
   &= Cov\left( {\sum\limits_{j =  - \infty }^\infty  {{\psi _j}{w_{t - j}}} ,\sum\limits_{j =  - \infty }^\infty  {{\psi _j}{w_{t + h - j}}} } \right) \\
   &= \sum\limits_{j =  - \infty }^\infty  {{\psi _j}{\psi _{j + h}}Cov\left( {{w_{t - j}},{w_{t - j}}} \right)}  \\
   &= \sigma _w^2\sum\limits_{j =  - \infty }^\infty  {{\psi _j}{\psi _{j + h}}}  \\ 
\end{aligned} \]

Within the above derivation, the key is to realize that 
$Cov\left( {{w_{t - j}},{w_{t + h - j}}} \right) = 0$ if $t - j \ne t + h - j$.

Lastly, one of the better formalities of a linear process is that it is able 
to be represented in a simplified form under the **backshift operator**:

\[{X_t} = \psi \left( B \right){W_t}\]

### Example: White Noise

The white noise process $\left\{X_t\right\}$, defined in \@ref(wn),
can be expressed as a linear process under:

\[\psi _j = \begin{cases}
      1 , &\mbox{ if } j = 0\\
      0 , &\mbox{ if } |j| \ge 1
\end{cases}.\]

and $\mu = 0$.

Therefore, $\left\{X_t\right\} \sim WN(0, \sigma^2_W)$

### Example: Moving Average Order 1

Similarly, consider $\left\{X_t\right\}$ to be a MA(1) process, 
given by \@ref(ma1). The process can be expressed linearly under: 

\[\psi _j = \begin{cases}
      1, &\mbox{ if } j = 0\\
      \theta , &\mbox{ if } j = 1 \\
      0, &\mbox{ if } j \ge 2
\end{cases}.\]

and $\mu = 0$.

Thus, we have: $X_t = W_t + \theta W_{t-1}$

### Example: Symmetric Moving Average

Consider a symmetric moving average given by:

\[{X_t} = \frac{1}{{2q + 1}}\sum\limits_{j =  - q}^q {{W_{t + j}}} \]

Thus, $\left\{X_t\right\}$ is defined for $q + 1 \le t \le n-q$. The above process
would be a linear process since:

\[\psi _j = \begin{cases}
      \frac{1}{{2q + 1}} , &\mbox{ if } -q \le j \le q\\
      0 , &\mbox{ if } |j| > q
\end{cases}.\]

and $\mu = 0$.

In practice, if $q = 1$, we would have:

\[{X_t} = \frac{1}{3}\left( {{W_{t - 1}} + {W_t} + {W_{t + 1}}} \right)\]

### Example: Autoregressive Process of Order 1

A more intensive application of a linear process is $\left\{X_t\right\}$ as an
AR1 process, defined in \@ref(ar1). The intensity comes
from the necessity to define the weights with respect
to the time lag.

\[\psi _j = \begin{cases}
      \phi^j , &\mbox{ if } j \ge 0\\
      0 , &\mbox{ if } j < 0
\end{cases}.\]

and $\mu = 0$.

Under the condition that $\left| \phi \right| < 1$ the
process can be considered to be the traditional $X_t = \phi X_{t-1} + W_t$. Furthermore, the process can also be considered to be an MA($\infty$)!
